src/Find_tree_stack.thy
@@ -1,19 +1,20 @@
-theory Find_tree_stack imports Tree_stack "~~/src/HOL/Library/Code_Target_Nat" begin
+theory Find_tree_stack imports Prelude Tree_stack "~~/src/HOL/Library/Code_Target_Nat" begin
 
-(* the search key is not really needed - it is a parameter of all these defns *)
-datatype fts_focus_t = Focus "key * key option * Tree * key option"
+(* the search key is not really needed - it is a parameter of all these defns; the xs and zs are the other leaves not in t *)
+datatype fts_focus_t = Focus "key * leaves_t * key option * Tree * key option * leaves_t" (* k,xs,l,t,u,zs *)
+
 
 type_synonym fts_state_t = "fts_focus_t * tree_stack_t"
 
-definition dest_fts_focus :: "fts_focus_t \<Rightarrow> key * key option * Tree * key option" where 
-"dest_fts_focus f = (case f of Focus(k,l,t,u) \<Rightarrow> (k,l,t,u))"
+definition dest_fts_focus :: "fts_focus_t \<Rightarrow> key * leaves_t * key option * Tree * key option * leaves_t" where 
+"dest_fts_focus f = (case f of Focus(k,xs,l,t,u,zs) \<Rightarrow> (k,xs,l,t,u,zs))"
 
-lemma dest_fts_focus_def_2: "dest_fts_focus (Focus(k,l,t,u)) = (k,l,t,u)"
+lemma dest_fts_focus_def_2: "dest_fts_focus (Focus(k,xs,l,t,u,zs)) = (k,xs,l,t,u,zs)"
 apply(simp add: dest_fts_focus_def)
 done
 
 definition tree_to_fts :: "key => Tree => fts_state_t" where
-"tree_to_fts k t = (Focus(k,None,t,None),Nil)"
+"tree_to_fts k t = (Focus(k,[],None,t,None,[]),[])"
 
 
 (*
@@ -37,9 +38,9 @@ its not just that lu is a bound, it is that the subtree is the unique subtree wh
 
 definition wellformed_fts_focus :: "key \<Rightarrow> ms_t \<Rightarrow> fts_focus_t => bool" where
 "wellformed_fts_focus k0 ms f = (
-  let (k,l,t,u) = dest_fts_focus f in
+  let (k,xs,l,t,u,zs) = dest_fts_focus f in
   let b1 = wellformed_tree ms t in
-  let b2 = check_keys l (set (k#(keys t))) u in
+  let b2 = check_keys_2 (xs|>leaves_to_map|>dom) l (set (k#(keys t))) u (zs|>leaves_to_map|>dom) in
   b1&b2&(k=k0))"
 
 (*end wf fts focus definition*)
@@ -52,8 +53,8 @@ definition wellformed_fts_1 :: "fts_state_t => bool" where
   case ts of
   Nil => True
   | cn#xs => (    
-    let (k,l,t,u) = dest_fts_focus f in
-    let (_,_,rs,i,_) = dest_cnode cn in
+    let (k,xs,l,t,u,zs) = dest_fts_focus f in
+    let (_,_,_,rs,i,_,_) = dest_cnode cn in
     let b0 = (t = rs!i) in
     let b2 = (cnode_to_bound cn = (l,u)) in  (* ensure bounds are linked *)
     b0&b2)
@@ -80,15 +81,18 @@ definition wellformed_fts :: "key \<Rightarrow> fts_state_t => bool" where
 definition step_fts :: "fts_state_t => fts_state_t option" where
 "step_fts fts = (
   let (f,ts) = fts in
-  let (k,l,t,u) = dest_fts_focus f in
+  let (k,xs,l,t,u,zs) = dest_fts_focus f in
   case t of Leaf kvs => None
   | Node(ks,rs) => (
     let i = search_key_to_index ks k in
-    let cn = Cnode(l,ks,rs,i,u) in
+    let cn = Cnode(xs,l,ks,rs,i,u,zs) in
     let ts2 = (cn # ts) in
     let t2 = rs!i in
     let (l2,u2) = cnode_to_bound cn in
-    let f2 = Focus(k,l2,t2,u2) in
+    let indexes_to_leaves = % is. is |> List.map (% j. tree_to_leaves (rs!j)) |> List.concat in
+    let xs' = (from_to 0 (i-1)) |> indexes_to_leaves in
+    let zs' = (from_to (i+1) (ks_to_max_child_index ks)) |> indexes_to_leaves in
+    let f2 = Focus(k,xs@xs',l2,t2,u2,zs'@zs) in
     Some(f2,ts2) ))
 "
 
@@ -97,7 +101,7 @@ definition step_fts :: "fts_state_t => fts_state_t option" where
 definition fts_reass :: "fts_state_t \<Rightarrow> Tree" where
 "fts_reass fts = (
   let (f,ts) = fts in
-  let (k,l,t,u) = dest_fts_focus f in
+  let (k,xs,l,t,u,zs) = dest_fts_focus f in
   reass t ts
 )"
 
@@ -112,6 +116,7 @@ definition invariant_wf_fts :: "bool" where
 (*end find invariant*)
 
 (* prefer lem2; k0 is located in the focus; proof by induction on ts; perhaps better to do this for the step case explicitly?*)
+(*
 definition lem1 :: "bool" where
 "lem1 = (
   ! k0 f ts.
@@ -122,8 +127,12 @@ definition lem1 :: "bool" where
   k0 : tree_to_map (Node(ks,rs)) |> dom \<longrightarrow>
   k0 : tree_to_map t |> dom 
 )"
+*)
 
-definition lem2 :: "bool" where
+(* for find, the following is all we need, but may be preferable to prove something stronger needed
+for insert and delete *)
+(*
+definition lem2 :: "bool" where you all very much for coming the other night: it was great to see you. Sadly we got a bit carried away by the liberation of not having a baby-sitter to get back to. Did at least
 "lem2 = (! k0 f ts f' ts'.
   let (_,_,t,_) = dest_fts_focus f in
   let (_,_,t',_) = dest_fts_focus f' in
@@ -132,18 +141,85 @@ definition lem2 :: "bool" where
   (step_fts (f,ts) = Some(f',ts')) \<longrightarrow>
   k0 : (t'|>tree_to_map|>dom)
 )"
+*)
 
+(* want to talk about all the leaves... *)
+(*
+definition lem3 :: "bool" where
+"lem3 = (! k0 f ts f' ts'.
+  let (_,_,t,_) = dest_fts_focus f in
+  let (_,_,t',_) = dest_fts_focus f' in
+  wellformed_fts k0 (f,ts) &
+  k0 : (t|>tree_to_map|>dom) &
+  (step_fts (f,ts) = Some(f',ts')) \<longrightarrow>
+  k0 : (t'|>tree_to_map|>dom)
+)"
+*)
 
-definition lemma_fts_reass :: "bool" where
-"lemma_fts_reass = (! k0 f ts.
+(* this still talks about the focus
+definition lem5 :: "bool" where
+"lem5 = (! k0 f ts.
   wellformed_fts k0 (f,ts) \<longrightarrow> (
   let (k,_,t,_) = dest_fts_focus f in
   ? xs zs. 
     let t' = fts_reass (f,ts) in 
     (t' |> tree_to_leaves = xs@(tree_to_leaves t)@zs) & 
     (k0 : tree_to_map t' |> dom \<longrightarrow> k0 : tree_to_map t |> dom))
+)"
+*)
+
+(* the lu separate leaves of focus from other leaves of reass *)
+definition lem6 :: "bool" where
+"lem6 = (! k0 f ts.
+  wellformed_fts k0 (f,ts) \<longrightarrow> (
+    let (k,xs,l,t,u,zs) = dest_fts_focus f in
+    ? xs zs. (
+      let t' = fts_reass (f,ts) in 
+      (t' |> tree_to_leaves = xs@(tree_to_leaves t)@zs) & 
+      (* note None is functioning as +-infinity here, rather than <<dont care>> *)
+      check_keys_2 (xs |> leaves_to_map|>dom) l {} u (zs|>leaves_to_map|>dom)))
 )"  
 
+
+(* following should say that if we start with xs=zs={}, then the xs@(leaves of the focus)@zs are the leaves
+of the original tree - ie the leaves are invariant; then we know the ordering on xs,leaves,zs, and we
+also know the bound lu 
+
+first show that step preserves wellformedness; then show it preserves leaves and check_keys_2
+
+*)
+
+definition lem7 :: "bool" where
+"lem7 = (! f trns k0 t0 ts0 f0.
+  (trns = { (s,s'). case s of None \<Rightarrow> s'=None | Some fts \<Rightarrow> step_fts fts = s' }) &
+  f : (trace_set trns) &
+  (tree_to_fts k0 t0 = (f0,ts0)) &
+  (Some(f0,ts0) = f 0) 
+  \<longrightarrow> (
+  ! (n::nat). case f n of None \<Rightarrow> True | Some fn \<Rightarrow> (
+  let (f_n,ts_n) = fn in
+  let (k,xs,l,t,u,zs) = dest_fts_focus f0 in
+  let (k,xs',l',t',u',zs') = dest_fts_focus f_n in
+  let ks' = t'|>tree_to_map|>dom in (
+  wellformed_fts k0 (f_n,ts_n)) \<longrightarrow> 
+  check_keys_2 (xs'|>leaves_to_map|>dom) l' ks' u' (zs'|>leaves_to_map|>dom) &
+  (xs'@(t'|>tree_to_leaves)@zs' = xs@(t|>tree_to_leaves)@zs))) 
+)"
+
+
+lemma btree_find_correct: "! trns f k0 t0 f0 ts0 v0.
+(trns = { (s,s'). case s of None \<Rightarrow> s'=None | Some fts \<Rightarrow> step_fts fts = s' }) &
+f : (trace_set trns) \<longrightarrow> (
+(tree_to_fts k0 t0 = (f0,ts0)) &
+(Some(f0,ts0) = f 0) &
+(tree_to_map t0 k0 = v0) \<longrightarrow> (
+! n f_n ts_n. (f (n::nat) = Some(f_n,ts_n)) \<longrightarrow>
+(let (k,xs,l,t,u,zs) = dest_fts_focus f_n in
+(tree_to_map t k0 = v0))))
+"
+sorry
+
+(* FIXME next step to look at insert, using a lem7-like lemma *)
 
 
 end
