src/Prelude.thy
@@ -20,4 +20,10 @@ lemma "maps_to_map_prop ms (maps_to_map ms)"
 definition leaves_to_map :: "('k * 'v) list list \<Rightarrow> ('k,'v) map" where
 "leaves_to_map ls = (image map_of (set ls)) |> maps_to_map"
 
+
+(* transition systems -------------------------------- *)
+
+definition trace_set :: "('s * 's) set \<Rightarrow> (nat \<Rightarrow> 's) set" where
+"trace_set trns = { f .  (! (n::nat). (f n, f(n+1)) : trns) }"
+
 end
